coq/ZF/Meta/Decl/Axiom/Replacement.v
@@ -1,0 +1,45 @@
+Require Import Coq.Lists.List.
+Require Import Coq.Strings.String.
+
+Require Import ZF.Meta.Env.
+Require Import ZF.Meta.Syntax.
+Require Import ZF.Meta.Term.Decl.
+Require Import ZF.Meta.Ty.
+
+Import ListNotations.
+
+Require Import ZF.Meta.Decl.Class.Relation.Functional.
+Require Import ZF.Meta.Decl.Set.OrdPair.
+
+(* forall F, Functional F ->                                                    *)
+(* forall a, exists b, forall y, y :< b <-> exists x, x :< a /\ F :(x,y):       *)
+Definition Replacement : DeclT :=
+  {| paraT := []
+  ;  resT  := TyProp
+  ;  bodyT :=
+      All VarTyClass
+        (Imp
+          (IdentT "Functional" [Var 0])
+          (All VarTySet
+            (Ex VarTySet
+              (All VarTySet
+                (Iff
+                  (Elem (Var 0) (Var 1))
+                  (Ex VarTySet
+                    (And
+                      (Elem (Var 0) (Var 3))
+                      (App
+                        (Var 4)
+                        (IdentT "ordPair" [Var 0; Var 1])))))))))
+  |}.
+
+Definition imports : Env := Env.unions
+  [ Functional.exports
+  ; OrdPair.exports
+  ].
+
+Definition exports : Env := Env.fromListT
+  [ ("Replacement"%string, Replacement)
+  ].
+
+Definition env : Env := Env.union imports exports.
